lulu

COQ/miniML.v
@@ -1,7 +1,11 @@
 (** miniML *)
 Require Import String.
 Open Scope string_scope.
+Require Import List.
+Open Scope list_scope.
+Import ListNotations. 
 
+Section miniML.
 (** représentation des termes *)
 
 Inductive terme :=
@@ -10,7 +14,16 @@ Inductive terme :=
 | Var : string -> terme
 | Nb : nat -> terme
 | Plus : terme -> terme -> terme
-| Et : terme -> terme -> terme .
+| Et : terme -> terme -> terme 
+| Si : terme -> terme -> terme -> terme
+| Tete : list terme -> terme
+| Liste : list terme -> terme
+| Cons : terme -> list terme -> terme
+| Reste : list terme ->  terme
+| Lambda: string -> terme -> terme
+| Fermeture : string -> terme -> list (string*terme) -> terme
+| App : terme -> terme -> terme
+.
 
 Inductive valeur : terme -> Prop := 
 | Nb_v : forall n:nat, valeur (Nb n)
@@ -19,49 +32,94 @@ Inductive valeur : terme -> Prop :=
 .
 
 (** représentation de l'environnement [\Gamma] *)
+Definition env := list (string * terme) .
 
-Definition env_init (ident:string):terme :=
-    match ident with
-    | "x" => Nb 1
-    | "y" => Nb 2
-    | "v" => Vrai 
-    | _ => Faux
+Definition env0 : env := [("x",Nb 1); ("y", Nb 2); ("v", Vrai)].
+Print env0.
+
+Fixpoint lookup (ident:string) (e:env):terme :=
+    match e with
+    | [] => Faux
+    | (x,y)::reste => if x =? ident then y else lookup ident reste
     end.
 
-    (** la sémantique *)
-Inductive sem: terme -> terme -> Prop  :=
-| r_vrai : sem Vrai Vrai
-| r_faux : sem Faux Faux
-| r_nb : forall n:nat, sem (Nb n) (Nb n)
-| r_var : forall x:string, sem (Var x) (env_init x)
-| r1_et : forall (e1 e2:terme) , sem e1 Faux  -> sem (Et e1 e2) Faux
-| r2_et : forall (e1 e2 v2:terme) , sem e1 Vrai  -> sem e2 v2 -> valeur v2 -> sem (Et e1 e2) v2
-| r_plus : forall (e1 e2:terme) (n1 n2:nat) , sem e1 (Nb n1) -> sem e2 (Nb n2) -> sem (Plus e1 e2) (Nb (n1+n2))
+
+(** la sémantique *)
+Inductive sem (e:env): terme -> terme -> Prop  :=
+| r_vrai : sem e Vrai Vrai
+| r_faux : sem e Faux Faux
+| r_nb : forall n:nat, sem e (Nb n) (Nb n)
+| r_var : forall x:string, sem e (Var x) (lookup x e)
+| r1_et : forall (t1 t2:terme) , sem e t1 Faux  -> sem e (Et t1 t2) Faux
+| r2_et : forall (t1 t2 v2:terme) , sem e t1 Vrai  -> sem e t2 v2 -> valeur v2 -> sem e (Et t1 t2) v2
+| r_plus : forall (t1 t2:terme) (n1 n2:nat) , sem e t1 (Nb n1) -> sem e t2 (Nb n2) -> sem e (Plus t1 t2) (Nb (n1+n2))
+| r_si_vrai : forall (t1 t2 v2 t3:terme), sem e t1 Vrai -> sem e t2 v2 -> valeur v2 -> sem e (Si t1 t2 t3) v2
+| r_si_faux : forall (t1 t2 t3 v3:terme), sem e t1 Faux -> sem e t3 v3 -> valeur v3 -> sem e (Si t1 t2 t3) v3
+(* fonctions sur liste*)
+| r_cons : forall (v1:terme) (l2: list terme), valeur v1 -> sem e (Cons v1 l2) (Liste (v1::l2))
+(* lambda expression *)
+| r_lambda : forall (x:string) (corps:terme), sem e (Lambda x corps) (Fermeture x corps e)
+(* application *)
+| r_app : forall (f corps t1 v1 w:terme) (x:string) (env1:env),
+    sem e f (Fermeture x corps env1) -> 
+    sem e t1 v1 ->
+    sem  ([(x,v1)] ++ env1) corps w ->
+    sem e (App f t1) w
 .
 
-(** le type des expressions *) 
 
-
-Lemma  test1 : sem (Var "x") (Nb 1) .
+Lemma  test1 : sem env0 (Var "x") (Nb 1) .
 apply r_var. Qed.
 
 Hint Constructors sem valeur .
 
-Lemma test3 : sem (Et Vrai Faux) Faux .
+Lemma test3 : sem env0 (Et Vrai Faux) Faux .
 apply r2_et. 
 auto. auto. auto.
 Qed.
 
-Lemma test2 : sem (Et Vrai (Et (Var "z") Vrai)) Faux.
+Lemma test2 : sem env0 (Et Vrai (Et (Var "z") Vrai)) Faux.
 apply r2_et.
 auto. apply r1_et.
 apply r_var. auto.
 Qed.
 
-Lemma test4 : sem (Et Vrai (Et (Var "v") Vrai)) Vrai.
+Lemma test4 : sem env0 (Et Vrai (Et (Var "v") Vrai)) Vrai.
 apply r2_et. repeat auto. apply r2_et. apply r_var. auto. auto. auto.
 Qed.
 
-Lemma test5 : sem (Plus (Nb 2) (Nb 5)) (Nb (2+5)).
+Lemma test5 : sem env0 (Plus (Nb 2) (Nb 5)) (Nb (2+5)).
 apply r_plus.  auto. auto.
 Qed.
+
+Lemma test6 : sem env0 (Si Vrai (Nb 3) (Nb 5)) (Nb 3).
+apply r_si_vrai. auto. auto. auto.
+Qed.
+
+Lemma t7 : sem env0 (Cons (Nb 5) [(Nb 6); (Nb 7)]) (Liste [(Nb 5); (Nb 6); (Nb 7)]).
+auto.
+Qed.
+
+Lemma t8 : exists t:terme, sem env0 (Cons (Nb 5) [(Nb 6); (Nb 7)]) t.
+eauto .
+Qed.
+
+Lemma t9 : {t:terme| sem env0 (Cons (Nb 5) [(Nb 6); (Nb 7)]) t}.
+eauto.
+Qed.
+
+Print t9.
+
+Definition succ : terme := Lambda "x" (Plus (Var "x") (Nb 1)).
+
+Lemma t10 : sem env0 (App succ (Nb 5)) (Nb 6).
+unfold succ.
+eapply r_app.
+eapply r_lambda.
+eapply r_nb.
+simpl.
+assert (sem [("x", Nb 1); ("y", Nb 2); ("v", Vrai); ("x", Nb 5)] (Var "x") (Nb 1)).
+eapply r_var.
+apply (r_plus 
+
+(*  r_plus : forall (t1 t2:terme) (n1 n2:nat) , sem e t1 (Nb n1) -> sem e t2 (Nb n2) -> sem e (Plus t1 t2) (Nb (n1+n2)) *)
